Make progress on pure_inferProgScript.sml

compiler/binary/pure_inferProgScript.sml
@@ -1,15 +1,15 @@
 (*
-  Translation of PureLang parser
+  Translation of PureLang type inferencer
  *)
 open basis
      pure_inferenceTheory
-     pure_backendProgTheory;
+     pure_parseProgTheory;
 
 val _ = new_theory "pure_inferProg";
 
-val _ = set_grammar_ancestry ["pure_backendProg", "pure_inference"];
+val _ = set_grammar_ancestry ["pure_parseProg", "pure_inference"];
 
-val _ = translation_extends "pure_backendProg";
+val _ = translation_extends "pure_parseProg";
 
 val _ = (max_print_depth := 1000);
 
@@ -145,12 +145,340 @@ val _ = (length (hyp r) = 0) orelse fail (); (* no side conditions *)
    pure_unify
  *-----------------------------------------------------------------------*)
 
+val _ = add_preferred_thy "-";
+
+Triviality PRECONDITION_INTRO:
+  (b ==> (x = y)) ==> (x = if PRECONDITION b then y else x)
+Proof
+  Cases_on `b` \\ SIMP_TAC std_ss [PRECONDITION_def]
+QED
+
+Triviality EXISTS_eq:
+  ∀xs. EXISTS P xs ⇔ MEMBER T (MAP P xs)
+Proof
+  fs [GSYM MEMBER_INTRO]
+  \\ Induct \\ fs []
+QED
+
+Theorem pure_vwalk_ind:
+   !P.
+      (!s v.
+        (!v1 u. FLOOKUP s v = SOME v1 /\ v1 = CVar u ==> P s u) ==>
+        P s v) ==>
+      (!s v. pure_wfs s ==> P s v)
+Proof
+  NTAC 3 STRIP_TAC
+  \\ Cases_on `pure_wfs s` \\ FULL_SIMP_TAC std_ss []
+  \\ HO_MATCH_MP_TAC
+     (pure_unificationTheory.pure_vwalk_ind
+       |> SPEC_ALL |> UNDISCH
+       |> Q.SPEC `P (s:num |-> itype)`
+       |> DISCH_ALL |> RW [AND_IMP_INTRO] |> GEN_ALL)
+  \\ fs []
+QED
+
+val r = translate
+ (pure_unificationTheory.pure_vwalk
+  |> SIMP_RULE std_ss [PULL_FORALL] |> SPEC_ALL
+  |> MATCH_MP PRECONDITION_INTRO)
+
+Theorem pure_vwalk_side_def:
+  ∀s v. pure_vwalk_side s v ⇔ pure_wfs s
+Proof
+  strip_tac \\ reverse $ Cases_on ‘pure_wfs s’ \\ fs []
+  >- simp [Once $ fetch "-" "pure_vwalk_side_def"]
+  \\ strip_tac
+  \\ first_assum mp_tac
+  \\ first_x_assum mp_tac
+  \\ qid_spec_tac ‘v’
+  \\ qid_spec_tac ‘s’
+  \\ ho_match_mp_tac pure_vwalk_ind
+  \\ rw [] \\ fs []
+  \\ simp [Once $ fetch "-" "pure_vwalk_side_def"]
+QED
+
+val _ = pure_vwalk_side_def |> update_precondition;
+
+val r = translate pure_unificationTheory.pure_walk;
+
+Theorem pure_walk_side[simp]:
+  ∀s t. pure_wfs s ⇒ pure_walk_side s t
+Proof
+  simp [Once $ fetch "-" "pure_walk_side_def"]
+QED
+
+Theorem pure_oc_ind:
+  ∀P. (∀v13 v14 v15.
+         (∀x9 x8 x7 x6 x5 x4 x3.
+            (pure_walk v13 v14 = TypeCons x9 x8 ⇒
+             ∀x1. MEM x1 x8 ⇒ P v13 x1 v15) ∧
+            (pure_walk v13 v14 = Tuple x7 ⇒ ∀x2. MEM x2 x7 ⇒ P v13 x2 v15) ∧
+            (pure_walk v13 v14 = Function x6 x5 ⇒
+             P v13 x6 v15 ∧ (¬pure_oc v13 x6 v15 ⇒ P v13 x5 v15)) ∧
+            (pure_walk v13 v14 = Array x4 ⇒ P v13 x4 v15) ∧
+            (pure_walk v13 v14 = M x3 ⇒ P v13 x3 v15)) ⇒
+         P v13 v14 v15) ⇒
+      ∀s t v. pure_wfs s ⇒ P s t v
+Proof
+  cheat
+QED
+
+(*
+  rpt strip_tac
+  \\ first_assum mp_tac
+  \\ first_x_assum mp_tac
+  \\ qid_spec_tac ‘v’
+  \\ qid_spec_tac ‘s’
+  \\ qid_spec_tac ‘t’
+  \\ cheat
+  \\ irule
+     pure_unificationTheory.pure_walkstar_ind
+     |> SIMP_RULE std_ss [PULL_FORALL] |> SPEC_ALL
+     |> Q.GEN ‘P’
+     |> Q.SPEC `P (s:num |-> itype)`
+     |> DISCH_ALL |> RW [AND_IMP_INTRO] |> GEN_ALL
+  REPEAT STRIP_TAC THEN Q.SPEC_TAC (`t`,`t`)
+  THEN IMP_RES_TAC unifyTheory.t_walkstar_ind
+  THEN POP_ASSUM HO_MATCH_MP_TAC THEN METIS_TAC []
+  *)
+
+val r = translate
+ (pure_unificationTheory.pure_oc
+  |> SIMP_RULE std_ss [PULL_FORALL,EXISTS_eq,MAP,MEMBER_def]
+  |> SPEC_ALL
+  |> MATCH_MP PRECONDITION_INTRO)
+
+Triviality pure_oc_side:
+  pure_oc_side s t v = pure_wfs s
+Proof
+  cheat
+QED
+
+val _ = pure_oc_side |> update_precondition;
+
+val r = translate pure_unificationTheory.pure_ext_s_check;
+
+Triviality pure_ext_s_check_side:
+  pure_ext_s_check_side s t v = pure_wfs s
+Proof
+  rewrite_tac [fetch "-" "pure_ext_s_check_side_def"]
+QED
+
+val _ = pure_ext_s_check_side |> update_precondition;
+
+Triviality pure_unify_lemma:
+  (pure_unify s t1 t2 =
+     if PRECONDITION (pure_wfs s) then
+      (case (pure_walk s t1,pure_walk s t2) of
+         (DBVar db1,DBVar db2) => if db1 = db2 then SOME s else NONE
+       | (DBVar db1,CVar v53) => pure_ext_s_check s v53 (DBVar db1)
+       | (PrimTy pty1,PrimTy pty2) => if pty1 = pty2 then SOME s else NONE
+       | (PrimTy pty1,CVar v73) => pure_ext_s_check s v73 (PrimTy pty1)
+       | (Exception,Exception) => SOME s
+       | (Exception,CVar v93) => pure_ext_s_check s v93 Exception
+       | (TypeCons c1 ts1,TypeCons c2 ts2) =>
+         if c1 = c2 then pure_unifyl s ts1 ts2 else NONE
+       | (TypeCons c1 ts1,CVar v113) =>
+         pure_ext_s_check s v113 (TypeCons c1 ts1)
+       | (Tuple ts1',Tuple ts2') => pure_unifyl s ts1' ts2'
+       | (Tuple ts1',CVar v133) => pure_ext_s_check s v133 (Tuple ts1')
+       | (Function t11 t12,Function t21 t22) =>
+         pure_unifyl s [t11; t12] [t21; t22]
+       | (Function t11 t12,CVar v153) =>
+         pure_ext_s_check s v153 (Function t11 t12)
+       | (Array t1,Array t2) => pure_unify s t1 t2
+       | (Array t1,CVar v173) => pure_ext_s_check s v173 (Array t1)
+       | (M t1',M t2') => pure_unify s t1' t2'
+       | (M t1',CVar v193) => pure_ext_s_check s v193 (M t1')
+       | (CVar v1,DBVar v214) => pure_ext_s_check s v1 (DBVar v214)
+       | (CVar v1,PrimTy v215) => pure_ext_s_check s v1 (PrimTy v215)
+       | (CVar v1,Exception) => pure_ext_s_check s v1 Exception
+       | (CVar v1,TypeCons v216 v217) =>
+         pure_ext_s_check s v1 (TypeCons v216 v217)
+       | (CVar v1,Tuple v218) => pure_ext_s_check s v1 (Tuple v218)
+       | (CVar v1,Function v219 v220) =>
+         pure_ext_s_check s v1 (Function v219 v220)
+       | (CVar v1,Array v221) => pure_ext_s_check s v1 (Array v221)
+       | (CVar v1,M v222) => pure_ext_s_check s v1 (M v222)
+       | (CVar v1,CVar v2) => SOME (if v1 = v2 then s else s |+ (v1,CVar v2))
+       | _ => NONE)
+     else pure_unify s t1 t2) ∧
+  (pure_unifyl s ts1 ts2 =
+     if PRECONDITION (pure_wfs s) then
+       case (ts1,ts2) of
+       | ([],[]) => SOME s
+       | (t1::ts1,t2::ts2) => (case pure_unify s t1 t2 of
+                               | NONE => NONE
+                               | SOME s' => pure_unifyl s' ts1 ts2)
+       | _ => NONE
+     else pure_unifyl s ts1 ts2)
+Proof
+  Cases_on ‘pure_wfs s’ \\ fs [PRECONDITION_def] \\ conj_tac
+  >- (drule_then (qspecl_then [‘t1’,‘t2’] mp_tac) pure_unificationTheory.pure_unify
+      \\ strip_tac \\ gvs [AllCaseEqs()])
+  \\ Cases_on ‘ts1’ \\ Cases_on ‘ts2’ \\ fs []
+  \\ fs [pure_unificationTheory.pure_unifyl_def]
+QED
+
+val r = translate_no_ind pure_unify_lemma;
+
+Triviality pure_unify_ind:
+  pure_unify_ind
+Proof
+  rewrite_tac [fetch "-" "pure_unify_ind_def"]
+  \\ cheat
+QED
+
+val _ = pure_unify_ind |> update_precondition;
+
+val pure_unify_ind_lemma =
+  pure_unify_ind |> REWRITE_RULE [fetch "-" "pure_unify_ind_def"];
+
+Triviality pure_unify_side:
+  (∀s t1 t2. pure_unify_side s t1 t2 ⇔ pure_wfs s) ∧
+  (∀s ts1 ts2. pure_unifyl_side s ts1 ts2 ⇔ pure_wfs s)
+Proof
+  cheat
+QED
+
+val _ = pure_unify_side |> update_precondition;
+
+Definition pure_unify_empty_def:
+  pure_unify_empty x y = pure_unify FEMPTY x y
+End
+
+val r = translate pure_unify_empty_def;
+
+Theorem pure_walkstar_ind:
+  ∀P. (∀v13 v14.
+         (∀x9 x8 x7 x6 x5 x4 x3.
+            (pure_walk v13 v14 = TypeCons x9 x8 ⇒ ∀x1. MEM x1 x8 ⇒ P v13 x1) ∧
+            (pure_walk v13 v14 = Tuple x7 ⇒ ∀x2. MEM x2 x7 ⇒ P v13 x2) ∧
+            (pure_walk v13 v14 = Function x6 x5 ⇒ P v13 x6 ∧ P v13 x5) ∧
+            (pure_walk v13 v14 = Array x4 ⇒ P v13 x4) ∧
+            (pure_walk v13 v14 = M x3 ⇒ P v13 x3)) ⇒
+         P v13 v14) ⇒
+      ∀s t. pure_wfs s ⇒ P s t
+Proof
+  cheat
+QED
+
+Triviality pure_walkstar_eta:
+  MAP (pure_walkstar s) = MAP $ λx. pure_walkstar s x
+Proof
+  AP_TERM_TAC \\ fs [FUN_EQ_THM]
+QED
+
+val r = translate
+ (pure_unificationTheory.pure_walkstar
+  |> SIMP_RULE std_ss [PULL_FORALL,EXISTS_eq,MAP,MEMBER_def]
+  |> SPEC_ALL
+  |> MATCH_MP PRECONDITION_INTRO
+  |> ONCE_REWRITE_RULE [pure_walkstar_eta]);
+
+Theorem pure_walkstar_side:
+  pure_walkstar_side s t = pure_wfs s
+Proof
+  cheat
+QED
+
+val _ = pure_walkstar_side |> update_precondition;
+
 (*-----------------------------------------------------------------------*
    solve
  *-----------------------------------------------------------------------*)
 
-val PRECONDITION_INTRO = Q.prove(
-  ‘(b ==> (x = y)) ==> (x = if PRECONDITION b then y else x)’,
-  Cases_on `b` THEN SIMP_TAC std_ss [PRECONDITION_def]);
+val r = translate is_solveable_def;
+val r = translate get_solveable_def;
+val r = translate activevars_def;
+val r = translate oreturn_def;
+val r = translate generalise_def;
+val r = translate monomorphise_implicit_def;
+val r = translate subst_constraint_def;
+
+Theorem subst_constraint_side:
+  ∀s t. subst_constraint_side s t = pure_wfs s
+Proof
+  ho_match_mp_tac subst_constraint_ind \\ rw []
+  \\ simp [Once $ fetch "-" "subst_constraint_side_def"]
+  \\ fs [fetch "-" "subst_vars_side_def"]
+QED
+
+val _ = subst_constraint_side |> update_precondition;
+
+Triviality infer_bind:
+  infer_bind (g : 'a inferM) f = λs.
+    case g s of
+    | NONE => NONE
+    | SOME (x, s') => (f x : 'b inferM) s'
+Proof
+  fs [infer_bind_def,FUN_EQ_THM]
+QED
+
+val r = translate
+  (solve_def |> RW [GSYM pure_unify_empty_def]
+   |> SIMP_RULE std_ss [infer_bind]);
+
+Theorem solve_side:
+  ∀s. solve_side s
+Proof
+  ho_match_mp_tac solve_ind \\ rw []
+  \\ simp [Once $ fetch "-" "solve_side_def"]
+  \\ rw [] \\ gvs []
+  \\ Cases_on ‘pure_unify_empty x29 x28’
+  \\ gvs [oreturn_def,fail_def,return_def]
+  \\ fs [pure_unify_empty_def]
+  \\ imp_res_tac pure_unificationTheory.pure_unify_wfs
+  \\ fs []
+QED
+
+val r = solve_side |> update_precondition;
+
+(*-----------------------------------------------------------------------*
+   top-level entry point
+ *-----------------------------------------------------------------------*)
+
+val r = translate pure_inferenceTheory.infer_top_level_def;
+
+val r = translate pure_typingTheory.freetyvars_ok_def;
+
+Triviality type_wf_eq:
+  type_wf typedefs v ⇔
+     case v of
+       TypeVar n => T
+     | PrimTy pty => T
+     | Exception => T
+     | TypeCons id tyargs =>
+       (EVERY I (MAP (λa. type_wf typedefs a) tyargs) ∧
+        case LLOOKUP typedefs id of
+        | NONE => F
+        | SOME (arity,constructors) => LENGTH tyargs = arity)
+     | Tuple ts => EVERY I (MAP (λa. type_wf typedefs a) ts)
+     | Function tf t => type_wf typedefs t ∧ type_wf typedefs tf
+     | Array t => type_wf typedefs t
+     | M t => type_wf typedefs t
+Proof
+  Cases_on ‘v’ \\ fs [pure_typingTheory.type_wf_def]
+  \\ fs [EVERY_MAP]
+  \\ rpt (CASE_TAC \\ fs []) \\ eq_tac \\ rw []
+QED
+
+val r = translate type_wf_eq;
+
+Definition every_pair_def:
+  every_pair P [] = T ∧
+  (every_pair P ((x,y)::xs) ⇔ P x y ∧ every_pair P xs)
+End
+
+Triviality intro_every_pair:
+  EVERY P xs ⇔ every_pair (λx y. P (x,y)) xs
+Proof
+  Induct_on ‘xs’ \\ fs [FORALL_PROD,every_pair_def]
+QED
+
+val r = translate (pure_inferenceTheory.typedefs_ok_impl_def
+          |> SIMP_RULE std_ss [intro_every_pair]);
+
+val r = translate pure_inferenceTheory.infer_types_def;
 
 val _ = export_theory ();
